substitution lemma, no partiality required

pulse/lib/steel/pulse/Pulse.Prover.Util.fsti
@@ -1,5 +1,7 @@
 module Pulse.Prover.Util
 
+open FStar.List.Tot
+
 open Pulse.Syntax
 open Pulse.Typing
 open Pulse.Checker.Common
@@ -11,73 +13,170 @@ module T = FStar.Tactics
 module RT = FStar.Reflection.Typing
 module Psubst = Pulse.Prover.Substs
 
-let subst_env_mk_env (f:RT.fstar_top_env) (ss:subst)
-  : Lemma (subst_env (mk_env f) ss == mk_env f)
-          [SMTPat (subst_env (mk_env f) ss)] = admit ()
+type nt_substs = l:list subst_elt { forall elt. L.memP elt l ==> NT? elt }
 
-let well_typed_ss (#g:env) (g':env) (ss:Psubst.t g) =
+let compose_nt_substs (ss1 ss2:nt_substs) : nt_substs =
+  assume (forall elt. L.memP elt (ss1@ss2) <==> (L.memP elt ss1 \/ L.memP elt ss2));
+  ss1 @ ss2
 
-  forall (x:var).{:pattern Set.mem x (Psubst.dom ss) }
-  Set.mem x (Psubst.dom ss) ==> (x `Set.mem` dom g' /\
-                                (let Some t = lookup g' x in
-                                 tot_typing g (Psubst.lookup ss x)
-                                              (Psubst.subst_term ss t)))
+let nt_subst_term (t:term) (ss:nt_substs) : term =
+  L.fold_left (fun t elt -> subst_term t [elt]) t ss
 
+let nt_subst_st_term (t:st_term) (ss:nt_substs) : st_term =
+  L.fold_left (fun t elt -> subst_st_term t [elt]) t ss
 
-let psubst_env (#g0:_) (g:env) (ss:Psubst.t g0) =
-  subst_env g (Psubst.as_subst ss)
+let nt_subst_comp (c:comp) (ss:nt_substs) : comp =
+  L.fold_left (fun c elt -> subst_comp c [elt]) c ss
 
-// different from extends, g1 may have dropped bindings from anywhere, not just the end
-let subenv (g1 g2:env) =
-  fstar_env g1 == fstar_env g2 /\
-  (forall (x:var).{:pattern Set.mem x (dom g1)}
-                  Set.mem x (dom g1) ==>
-                  (Set.mem x (dom g2) /\
-                   lookup g1 x == lookup g2 x))
+let nt_subst_env (g:env) (ss:nt_substs) : g':env { fstar_env g' == fstar_env g /\
+                                                   dom g' == dom g } =
+  admit ();
+  L.fold_left (fun g elt -> subst_env g [elt]) g ss
 
-let rec filter_ss (#g0:env) (g:env) (ss:Psubst.t g0)
-  : Tot (g':env { subenv g' g /\ Set.disjoint (dom g') (Psubst.dom ss) })
-        (decreases bindings g) =
+let rec nt_subst_term_compose (t:term) (ss1 ss2:nt_substs)
+: Lemma (ensures nt_subst_term (nt_subst_term t ss1) ss2 ==
+                 nt_subst_term t (compose_nt_substs ss1 ss2))
+        (decreases L.length ss1) =
 
-  match bindings g with
-  | [] -> mk_env (fstar_env g)
-  | _ ->
-    let ( x, t, g ) = remove_latest_binding g in
-    let g = filter_ss g ss in
-    if Set.mem x (Psubst.dom ss) then g
-    else push_binding g x ppname_default t
+match ss1 with
+| [] -> ()
+| (NT x e)::tl -> nt_subst_term_compose (subst_term t [ NT x e ]) tl ss2
 
-val push_subst_env (#g:_) (s1 s2:Psubst.t g) (g':env)
-  : Lemma (requires Set.disjoint (Psubst.dom s1) (Psubst.dom s2))
-          (ensures psubst_env g' (Psubst.push s1 s2) ==
-                   psubst_env (psubst_env g' s1) s2)
-          [SMTPat (psubst_env (psubst_env g' s1) s2)]
+let rec nt_subst_st_term_compose (t:st_term) (ss1 ss2:nt_substs)
+: Lemma (ensures nt_subst_st_term (nt_subst_st_term t ss1) ss2 ==
+                 nt_subst_st_term t (compose_nt_substs ss1 ss2))
+        (decreases L.length ss1) =
 
-val apply_partial_subs (#g0:env) (#t:st_term) (#c:comp_st)
-  (uvs:env { disjoint uvs g0 })
-  (ss:Psubst.t g0 { well_typed_ss uvs ss })
-  (t_typing:st_typing (push_env g0 uvs) t c)
+match ss1 with
+| [] -> ()
+| (NT x e)::tl -> nt_subst_st_term_compose (subst_st_term t [ NT x e ]) tl ss2
 
-  : uvs_unresolved:env { uvs_unresolved == filter_ss uvs ss } &
-    st_typing (push_env g0 (psubst_env uvs_unresolved ss))
-              (Psubst.subst_st_term ss t)
-              (Psubst.subst_comp ss c)
+let rec nt_subst_comp_compose (c:comp) (ss1 ss2:nt_substs)
+: Lemma (ensures nt_subst_comp (nt_subst_comp c ss1) ss2 ==
+                 nt_subst_comp c (compose_nt_substs ss1 ss2))
+        (decreases L.length ss1) =
 
-val apply_partial_subs_veq (#g0:env) (#p1 #p2:vprop)
-  (uvs:env { disjoint uvs g0 })
-  (ss:Psubst.t g0 { well_typed_ss uvs ss })
-  (veq:vprop_equiv (push_env g0 uvs) p1 p2)
+match ss1 with
+| [] -> ()
+| (NT x e)::tl -> nt_subst_comp_compose (subst_comp c [ NT x e ]) tl ss2
 
-  : uvs_unresolved:env { uvs_unresolved == filter_ss uvs ss } &
-    vprop_equiv (push_env g0 (psubst_env uvs_unresolved ss))
-                (Psubst.subst_term ss p1)
-                (Psubst.subst_term ss p2)
-
-let ghost_comp pre post : c:comp_st { comp_pre c == pre /\ comp_post c == post } = 
-  C_STGhost tm_emp_inames { u=u_zero; res=tm_unit; pre; post }
+let rec well_typed_ss (g:env) (uvs:env) (ss:nt_substs) : Tot Type0 (decreases L.length ss) =
+  match bindings uvs, ss with
+  | [], [] -> True
+  | _::_, (NT x e)::ss_rest ->
+    let y, ty, rest_uvs = remove_binding uvs in
+    x == y /\
+    tot_typing g e ty /\
+    well_typed_ss g (subst_env rest_uvs [ NT x e ]) ss_rest
+  | _, _ -> False
 
 
-val idem_steps (g:env) (ctxt:vprop)
-  : t:st_term &
-    st_typing g t (ghost_comp ctxt (tm_star (list_as_vprop (vprop_as_list ctxt))
-                                            tm_emp))
+let coerce_eq (#a #b:Type) (x:a) (_:squash (a === b)) : y:b{y == x} = x
+
+let rec st_typing_nt_substs
+  (g:env) (uvs:env) (g':env { pairwise_disjoint g uvs g' })
+  (#t:st_term) (#c:comp_st) (t_typing:st_typing (push_env g (push_env uvs g')) t c)
+  (ss:nt_substs { well_typed_ss g uvs ss })
+: Tot (st_typing (push_env g (nt_subst_env g' ss)) (nt_subst_st_term t ss) (nt_subst_comp c ss))
+      (decreases L.length ss) =
+
+match bindings uvs with
+| [] ->
+  assert (equal (push_env uvs g') g');
+  t_typing
+
+| _ ->
+  let x, ty, uvs' = remove_binding uvs in
+  let (NT y e)::ss' = ss in
+  let e_typing = FStar.IndefiniteDescription.elim_squash #(tot_typing g e ty) () in
+  push_env_assoc (singleton_env (fstar_env uvs) x ty) uvs' g';
+  let t_typing
+    : st_typing (push_env g (push_env (singleton_env (fstar_env g) x ty) (push_env uvs' g'))) t c
+    = coerce_eq t_typing () in
+  let t_typing
+    : st_typing (push_env g (subst_env (push_env uvs' g') [ NT y e ]))
+                (subst_st_term t [ NT y e ])
+                (subst_comp c [ NT y e ])
+    = st_typing_subst g x ty (push_env uvs' g') e_typing t_typing in
+
+  assume (subst_env (push_env uvs' g') [ NT y e ] ==
+          push_env (subst_env uvs' [ NT y e ]) (subst_env g' [ NT y e ]));
+
+  st_typing_nt_substs g
+    (subst_env uvs' [ NT y e ])
+    (subst_env g' [ NT y e ])
+    t_typing ss'
+
+
+
+
+// let subst_env_mk_env (f:RT.fstar_top_env) (ss:subst)
+//   : Lemma (subst_env (mk_env f) ss == mk_env f)
+//           [SMTPat (subst_env (mk_env f) ss)] = admit ()
+
+// let well_typed_ss (#g:env) (g':env) (ss:Psubst.t g) =
+
+//   forall (x:var).{:pattern Set.mem x (Psubst.dom ss) }
+//   Set.mem x (Psubst.dom ss) ==> (x `Set.mem` dom g' /\
+//                                 (let Some t = lookup g' x in
+//                                  tot_typing g (Psubst.lookup ss x)
+//                                               (Psubst.subst_term ss t)))
+
+
+// let psubst_env (#g0:_) (g:env) (ss:Psubst.t g0) =
+//   subst_env g (Psubst.as_subst ss)
+
+// // different from extends, g1 may have dropped bindings from anywhere, not just the end
+// let subenv (g1 g2:env) =
+//   fstar_env g1 == fstar_env g2 /\
+//   (forall (x:var).{:pattern Set.mem x (dom g1)}
+//                   Set.mem x (dom g1) ==>
+//                   (Set.mem x (dom g2) /\
+//                    lookup g1 x == lookup g2 x))
+
+// let rec filter_ss (#g0:env) (g:env) (ss:Psubst.t g0)
+//   : Tot (g':env { subenv g' g /\ Set.disjoint (dom g') (Psubst.dom ss) })
+//         (decreases bindings g) =
+
+//   match bindings g with
+//   | [] -> mk_env (fstar_env g)
+//   | _ ->
+//     let ( x, t, g ) = remove_latest_binding g in
+//     let g = filter_ss g ss in
+//     if Set.mem x (Psubst.dom ss) then g
+//     else push_binding g x ppname_default t
+
+// val push_subst_env (#g:_) (s1 s2:Psubst.t g) (g':env)
+//   : Lemma (requires Set.disjoint (Psubst.dom s1) (Psubst.dom s2))
+//           (ensures psubst_env g' (Psubst.push s1 s2) ==
+//                    psubst_env (psubst_env g' s1) s2)
+//           [SMTPat (psubst_env (psubst_env g' s1) s2)]
+
+// val apply_partial_subs (#g0:env) (#t:st_term) (#c:comp_st)
+//   (uvs:env { disjoint uvs g0 })
+//   (ss:Psubst.t g0 { well_typed_ss uvs ss })
+//   (t_typing:st_typing (push_env g0 uvs) t c)
+
+//   : uvs_unresolved:env { uvs_unresolved == filter_ss uvs ss } &
+//     st_typing (push_env g0 (psubst_env uvs_unresolved ss))
+//               (Psubst.subst_st_term ss t)
+//               (Psubst.subst_comp ss c)
+
+// val apply_partial_subs_veq (#g0:env) (#p1 #p2:vprop)
+//   (uvs:env { disjoint uvs g0 })
+//   (ss:Psubst.t g0 { well_typed_ss uvs ss })
+//   (veq:vprop_equiv (push_env g0 uvs) p1 p2)
+
+//   : uvs_unresolved:env { uvs_unresolved == filter_ss uvs ss } &
+//     vprop_equiv (push_env g0 (psubst_env uvs_unresolved ss))
+//                 (Psubst.subst_term ss p1)
+//                 (Psubst.subst_term ss p2)
+
+// let ghost_comp pre post : c:comp_st { comp_pre c == pre /\ comp_post c == post } = 
+//   C_STGhost tm_emp_inames { u=u_zero; res=tm_unit; pre; post }
+
+
+// val idem_steps (g:env) (ctxt:vprop)
+//   : t:st_term &
+//     st_typing g t (ghost_comp ctxt (tm_star (list_as_vprop (vprop_as_list ctxt))
+//                                             tm_emp))
